Put generic soundness proof, instantiate for exist and all path

coq/mixed_shallow/proofsystem.v
@@ -1,37 +1,25 @@
-Set Implicit Arguments.
-
 Section domain.
 Variable cfg : Set.
 
 Definition formula env : Type := env -> cfg -> Prop.
 Definition stateless env : Type := env -> Prop.
 (* Definition rule := { env : Type & formula env & formula env }. *)
+Definition system := forall env,
+  formula env -> formula env -> Prop.
 
-Inductive flag : Set := all_path | ex_path.
-Inductive rule (env : Type) : Type :=
-  Rule (f:flag) (phi phi':formula env).
-
-Definition system := forall env, rule env -> Prop.
-
-Definition in_opt_system (S : option system) : system :=
+Definition in_opt_system (S : option system) env (phi phi' : formula env) : Prop :=
   match S with
-    | None => fun _ _ => False
-    | Some sys => sys
+    | None => False
+    | Some sys => sys env phi phi'
   end.
 
-Definition empty_system : system := fun _ _ => False.
+Definition cons_system env (phi phi' : formula env) (S : system) : system :=
+  fun env0 X X0 =>
+    S env0 X X0 \/
+    {H : env = env0 | phi = eq_rect_r _ X H /\ phi' = eq_rect_r _ X0 H}.
 
-Definition cons_system env (r : rule env) (S : system) : system :=
-  fun env0 r' => S env0 r' \/ {H : env = env0 | r = eq_rect_r _ r' H}.
-
-Definition cons_opt_system env (r : rule env) (S : option system) : option system :=
-  Some (cons_system r (in_opt_system S)).
-
-Definition system_opt (C : option system) : system :=
-  match C with
-    | None => empty_system
-    | Some s => s
-  end.
+Definition cons_opt_system env (phi phi' : formula env) (S : option system) : option system :=
+  Some (cons_system env phi phi' (in_opt_system S)).
 
 Definition system_empty (S : option system) : Prop :=
   match S with
@@ -39,63 +27,67 @@ Definition system_empty (S : option system) : Prop :=
     | None => True
   end.
 
-Definition union_system (S1 S2 : system) : system :=
-  fun env r => S1 env r \/ S2 env r.
+Definition union_system (C : option system) (S : system) : system :=
+  match C with
+    | None => S
+    | Some S1 =>
+      fun env0 X X0 => S1 env0 X X0 \/ S env0 X X0
+  end.
   
-(* accepts a rule if valid in the system *)
-(*
+(* accepts a rule if all instances come from the relation *)
 Definition system_of_relation (R : cfg -> cfg -> Prop) : system :=
-*)
+  fun env phi phi' =>
+    forall (rho : env) gamma gamma',
+      phi rho gamma -> phi' rho gamma' -> R gamma gamma'.
 
 Section FixTransition.
 Variable (S : cfg -> cfg -> Prop).
 
-Inductive IS (C : option system) (A : system) : forall env, rule env -> Prop :=
-  | is_all_step : forall env (phi phi' : formula env),
-                    (forall e c, phi e c ->
-                                 (exists c2, S c c2) /\
-                                 (forall c2, S c c2 -> phi' e c2)) ->
-                    IS C A (Rule all_path phi phi')
-  | is_ex_step : forall env (phi phi' : formula env),
-                   (forall e c, phi e c -> exists c2, S c c2 /\ phi' e c2) ->
-                   IS C A (Rule ex_path phi phi')
-  | is_axiom : forall env r, A env r -> IS C A r
-  | is_refl : forall env f phi, system_empty C -> IS C A (@Rule env f phi phi)
-  | is_trans : forall env f (phi phi' phi'' : formula env),
-       IS C A (Rule f phi phi') ->
-       IS None (union_system A (system_opt C)) (Rule f phi' phi'') ->
-       IS C A (Rule f phi phi'')
-  | is_conseq : forall f env 
+Inductive IS (C : option system) (A : system) : forall env,
+  formula env -> formula env -> Prop :=
+  | is_step : forall env (phi phi' : formula env),
+                (forall e c, phi e c ->
+                             (exists c2, S c c2) /\
+                             (forall c2, S c c2 -> phi' e c2)) ->
+                 IS C A env phi phi'
+  | is_axiom : forall env phi phi',
+                 A env phi phi' -> IS C A env phi phi'
+  | is_refl : forall env phi, system_empty C -> IS C A env phi phi
+  | is_trans : forall env phi phi' phi'',
+       IS C A env phi phi' ->
+       IS None (union_system C A) env phi' phi'' ->
+       IS C A env phi phi''
+  | is_conseq : forall env 
        (phi1 phi1' phi2 phi2' : formula env),
        (forall e g, phi1 e g -> phi1' e g) ->
        (forall e g, phi2 e g -> phi2' e g) ->
-       IS C A (Rule f phi1' phi2) ->
-       IS C A (Rule f phi1 phi2')
-  | is_case : forall env f phi phi1 phi',
-       IS C A (@Rule env f phi  phi') ->
-       IS C A (Rule f phi1 phi') ->
-       IS C A (Rule f (fun e g => phi e g \/ phi1 e g) phi')
+       IS C A env phi1' phi2 ->
+       IS C A env phi1 phi2'
+  | is_case : forall env phi phi1 phi',
+       IS C A env phi  phi' ->
+       IS C A env phi1 phi' ->
+       IS C A env (fun e g => phi e g \/ phi1 e g) phi'
 (* use embedding projection pair -
    have env, env' bigger,
    env' phi (fun e' => phi' (project e'))
    env (fun e => exists e', extends e e' /\ phi e') phi'
   *)
-  | is_abstr : forall f env denx
+  | is_abstr : forall env denx
        (phi : formula (env * denx)) (phi' : formula env),
-       IS C A (@Rule (env * denx) f phi (fun rho_and_x g => phi' (fst rho_and_x) g)) ->
-       IS C A (Rule f (fun rho g => exists x, phi (rho , x) g) phi')
-  | is_circ : forall env f phi phi',
-       IS (cons_opt_system (Rule f phi phi') C) A (@Rule env f phi phi') ->
-       IS C A (Rule f phi phi')
-  | is_subst : forall env env' flg (f : env -> env') (phi phi' : formula env'),
-       IS C A (Rule flg phi phi') ->
-       IS C A (Rule flg (fun e g => phi (f e) g) (fun e g => phi' (f e) g))
-  | is_lf : forall env f phi phi' psi,
-       IS C A (@Rule env f phi phi') ->
-       IS C A (Rule f (fun e g => phi e g  /\ psi e)
-                      (fun e g => phi' e g /\ psi e)).
+       IS C A (env * denx) phi (fun rho_and_x g => phi' (fst rho_and_x) g) ->
+       IS C A env (fun rho g => exists x, phi (rho , x) g) phi'
+  | is_circ : forall env phi phi',
+       IS (cons_opt_system env phi phi' C) A env phi phi' ->
+       IS C A env phi phi'
+  | is_subst : forall env env' f phi phi',
+       IS C A env' phi phi' ->
+       IS C A env (fun e g => phi (f e) g) (fun e g => phi' (f e) g)
+  | is_lf : forall env phi phi' psi,
+       IS C A env phi phi' ->
+       IS C A env (fun e g => phi e g  /\ psi e)
+                  (fun e g => phi' e g /\ psi e).
 
-(*
+
 Section StepGood.
 Variable (Ssys : system).
 Hypothesis (Ssys_welldef :
@@ -148,7 +140,6 @@ destruct H0 as (env & phi & phi' & e2 & Hssys & Hphi & Hphi').
 apply (H env phi phi' Hssys e2 Hphi c2 Hphi').
 Qed.
 End StepGood.
-*)
 End FixTransition.
 
 End domain.
