coq/mixed_shallow/generic_ex.v
@@ -1,0 +1,293 @@
+Require Import generic_soundness.
+
+Add LoadPath "../ml_proof".
+
+Require Import reduction.
+
+Require Import proofsystem.
+Set Implicit Arguments.
+
+Require Import Setoid.
+Require Import Relation_Definitions.
+
+Axiom cfg : Set.
+Axiom S : cfg -> cfg -> Prop.
+
+(* Lemmas *)
+Lemma clos_lift (A B : Type) (R1 : relation A) (R2 : relation B)
+  (f : B -> A) :
+  (forall x y, R1 x y -> forall x', x = f x' -> exists y', R2 x' y' /\ y = f y') ->
+  forall strict x y,
+  clos R1 strict x y ->
+  forall x', x = f x' ->
+  exists y', clos R2 strict x' y' /\ y = f y'.
+induction 2;intros;
+repeat match goal with
+         | [H : _ -> _ -> ?R _ _ -> _, H1 : ?R _ _ |- _] => specialize (H _ _ H1)
+         | [H : forall x, ?a = f x -> _, H1 : ?a = f _ |- _] => specialize (H _ H1)
+         | [H : exists y', _ /\ _ = f y' |-_] =>
+           destruct H as [? []]
+       end;
+eauto using clos.
+Qed.
+
+Lemma terminates_next : forall {A : Set} {R : relation A} (a : A),
+  terminates a R -> forall b, R a b -> terminates b R.
+destruct 1.
+assumption.
+Qed.
+
+Lemma under_terminates : forall {A : Set} {R : relation A} (a : A),
+  terminates a R -> forall (P : A -> Prop),
+  (forall a0, clos R false a a0 ->
+              (forall a', R a0 a' -> P a') ->
+              P a0)
+  -> P a.
+intros A R a term P.
+move term after P.
+induction term as [a HAcc IH].
+intro Hlater.
+apply Hlater.
+constructor.
+intros a' Raa.
+apply IH.
+assumption.
+intros a0 Ha'a0 Hnext.
+apply Hlater.
+clear -Raa Ha'a0. eauto using clos.
+assumption.
+Qed.
+
+Lemma clos_cat'
+     : forall (A : Type) (R : relation A) (a : A) (s1 : bool) 
+         (b : A) (s2 s3 : bool) (c : A),
+       clos R s1 a b -> clos R s2 b c -> implb s3 (s1 || s2) = true -> clos R s3 a c.
+intros.
+pose proof (clos_cat H H0) as H2; clear -H1 H2.
+destruct s3. simpl in H1; rewrite H1 in H2;assumption.
+destruct (orb s1 s2);auto using clos_unstrict.
+Qed.
+
+Module ExPathSemantics <: ReachabilitySemantics.
+
+(* Definitions *)
+Definition index : Set := {gamma : cfg | terminates gamma S}.
+Definition ix_rel (i1 i2 : index) : Prop :=
+  S (proj1_sig i1) (proj1_sig i2).
+
+Definition holds' strict env (phi phi' : formula cfg env) : cfg -> Prop :=
+  fun parent =>
+    forall rho gamma1,
+      clos S false parent gamma1 ->
+      phi rho gamma1 ->
+      exists gamma2, clos S strict gamma1 gamma2 /\ phi' rho gamma2.
+Definition holds strict env phi1 phi2 (i : index) := @holds' strict env phi1 phi2 (proj1_sig i).
+
+(* Nontrivial proofs *)
+(** Circularity **)
+Lemma ix_rel_ind : forall env (phi phi' : formula cfg env),
+      forall i0,
+      (forall i, clos ix_rel false i0 i ->
+                   (forall i', ix_rel i i' -> holds true phi phi' i') ->
+                   holds true phi phi' i)
+       -> holds true phi phi' i0.
+intros env phi phi' i Hix_later.
+destruct i as [a Hterm].
+unfold holds. simpl.
+apply (under_terminates Hterm).
+intros a0 Haa0 Hnext.
+
+assert (exists i', clos ix_rel false (exist _ a Hterm) i' /\ a0 = proj1_sig i').
+  clear -Haa0. apply clos_lift with (R1:=S) (x:=a);[|assumption|reflexivity].
+  intros.
+  destruct x';simpl in *|- *;subst.
+  assert (terminates y S) by (destruct t as [H0]; apply H0; assumption).
+  exists (exist _ y H0). split;[|reflexivity].
+  unfold ix_rel;simpl. assumption.
+destruct H as [i' [Hreach Hend]].
+specialize (Hix_later i' Hreach).
+rewrite Hend.
+apply Hix_later.
+intros.
+apply Hnext.
+rewrite Hend.
+exact H.
+Qed.
+
+Create HintDb holds_solve discriminated.
+Hint Transparent holds holds' : holds_solve.
+Hint Unfold holds' : holds_solve.
+
+Ltac clear_except_path :=
+repeat match goal with
+  | [H : ?Hyp |- _] =>
+    match Hyp with
+      | terminates _ _ => fail 1
+      | clos _ _ _ _ => fail 1
+      | S ?x ?y => apply (clos_step _ true) in H
+      | _ => clear H
+    end
+  end.
+Ltac clos_solve :=
+  clear_except_path;
+match goal with
+  | [|- clos _ false ?x ?x] => apply clos_refl
+  | [|- clos _ false _ _] =>
+    repeat match goal with
+             | [H : clos _ true _ _ |- _] => apply clos_unstrict in H
+           end;
+    repeat match goal with
+             | [H : clos ?S _ ?x ?y |- clos ?S _ ?x ?y ] => assumption
+             | [H : clos ?S _ ?x ?y, H2 : clos ?S _ ?y _ |- clos ?S _ ?x _ ] =>
+               pose proof (clos_trans H H2); clear H2
+           end
+  | [|- clos _ _ _ _] =>
+    repeat match goal with
+         | [H : clos ?S ?f ?x ?y |- clos ?S ?f ?x ?y ] => assumption
+         | [H : clos ?S true ?x ?y, H2 : clos ?S _ ?y _ |- clos ?S _ ?x _ ] =>
+           pose proof (clos_cons_lt H H2); clear H H2
+         | [H : clos ?S _ ?x ?y, H2 : clos ?S true ?y _ |- clos ?S _ ?x _ ] =>
+           pose proof (clos_cons_rt H H2); clear H H2
+      end
+end.
+
+Hint Extern 0 (clos _ _ _ _) => clos_solve : holds_solve.
+
+Ltac holds_start := intros;
+  repeat match goal with
+  (* open unnecessary uses of holds/indices *)
+  | [i : index |- _] => destruct i
+  | [H : holds _ _ _ (exist _ _ _) |- _] => unfold holds in H;simpl proj1_sig in H
+  | [|- holds _ _ _ (exist _ _ _)] => unfold holds;simpl proj1_sig;unfold holds';intros
+  | [H : ix_rel (exist _ _ _) _ |- _] => unfold ix_rel in H; simpl proj1_sig in H
+  | [H : ix_rel _ (exist _ _ _) |- _] => unfold ix_rel in H; simpl proj1_sig in H
+  (* Instantate a hypothesis quantified over ix_rel, as appears in strict trans *)
+  | [H : forall i', ix_rel (exist _ ?x ?t) i' -> holds _ ?phi _ i',
+       Hphi : ?phi _ ?x0 |- _ ] =>
+    let Hprog := fresh "Hprog" in
+    assert (clos S true x x0) as Hprog by clos_solve;
+    let x1 := fresh "x1" with Hstep := fresh "Hstep" with Hreach := fresh "Hreach" in
+    apply clos_true_step in Hprog; destruct Hprog as [x1 [Hstep Hreach]];
+    specialize (H (exist _ x1 (terminates_next t _ Hstep)) Hstep)
+  (* Use holds' hypotheses *)
+  | [H : holds' _ ?phi _ ?x, Hphi : ?phi _ ?gamma |- _]=>
+    let Hreach := fresh "Hreach" in
+    assert (clos S false x gamma) as Hreach by clos_solve;
+    specialize (H _ _ Hreach Hphi)
+  | [H : exists _, clos S _ _ _ /\ _ |- _] => destruct H as [? []]
+  end.
+Ltac holds_finish :=
+  solve[eauto with holds_solve
+       |intuition
+          (repeat match goal with
+             | [H : forall _ _, ?phi _ _ -> _, Hphi : ?phi _ _ |- _] =>
+               specialize (H _ _ Hphi)
+           end;firstorder with holds_solve)
+       ].
+Ltac holds_tac := holds_start;holds_finish.
+
+(** Transitivity **)
+Lemma holds_trans_strict : forall env phi phi' phi'' i,
+    @holds true env phi phi' i ->
+    (forall i' : index, ix_rel i i' -> holds false phi' phi'' i') ->
+   holds true phi phi'' i.
+holds_tac.
+Qed.
+
+Lemma holds_trans : forall env phi phi' phi'' i,
+    @holds false env phi phi' i ->
+    holds false phi' phi'' i ->
+    holds false phi phi'' i.
+holds_tac.
+Qed.
+
+Lemma holds_strict_later : forall env phi1 phi2 i,
+                             @holds true env phi1 phi2 i ->
+                             forall i', ix_rel i i' ->
+                                        holds true phi1 phi2 i'.
+holds_tac.
+Qed.
+
+Lemma holds_unstrict : forall env phi1 phi2 i,
+                         @holds true env phi1 phi2 i -> holds false phi1 phi2 i.
+holds_tac.
+Qed.
+
+Lemma holds_step : forall env (phi phi' : formula cfg env),
+    (forall (e : env) (c : cfg),
+      phi e c ->
+      (exists c2 : cfg, S c c2) /\ (forall c2 : cfg, S c c2 -> phi' e c2)) ->
+    forall i, holds true phi phi' i.
+holds_tac.
+Qed.
+
+Lemma holds_refl : forall env phi i, @holds false env phi phi i.
+holds_tac.
+Qed.
+
+Lemma holds_case :
+    forall strict env (phi phi1 phi' : formula cfg env) i,
+      holds strict phi phi' i -> holds strict phi1 phi' i ->
+      holds strict (fun (e : env) (g : cfg) => phi e g \/ phi1 e g) phi' i.
+holds_tac.
+Qed.
+
+Lemma holds_mut_conseq :
+    forall strict env1 (phi1 phi2 : formula cfg env1)
+                  env2 (phi1' phi2' : formula cfg env2),
+     (forall gamma rho,
+        phi1 rho gamma ->
+        exists rho', phi1' rho' gamma /\
+                     forall gamma', phi2' rho' gamma' -> phi2 rho gamma') ->
+    forall i, holds strict phi1' phi2' i ->
+              holds strict phi1 phi2 i.
+holds_tac.
+Qed.
+
+Definition cfg := cfg.
+Definition S := S.
+End ExPathSemantics.
+
+Module ExPathSoundness := Soundness ExPathSemantics.
+
+Definition holds strict env (phi phi' : formula cfg env) :=
+  forall rho gamma, terminates gamma S ->
+    phi rho gamma -> exists gamma', phi' rho gamma' /\ clos S strict gamma gamma'.
+
+Lemma approx_holds env (phi phi' : formula cfg env) strict :
+  (forall i, ExPathSemantics.holds strict phi phi' i) ->
+  holds strict phi phi'.
+intro H. unfold holds.
+intros.
+specialize (H (exist _ gamma H0) _ _ (clos_refl _ _) H1).
+firstorder.
+Qed.
+
+Lemma holds_approx env (phi phi' : formula cfg env) strict :
+  holds strict phi phi' ->
+  (forall i, ExPathSemantics.holds strict phi phi' i).
+intros Hstrong i.
+destruct i as [gamma term].
+unfold ExPathSemantics.holds, ExPathSemantics.holds'.
+intros rho gamma1 Hreach Hphi.
+specialize (Hstrong _ gamma1 (terminates_fwd term Hreach) Hphi).
+firstorder.
+Qed.
+
+Definition system_holds (A : system cfg) :=
+  forall env phi1 phi2, @A env phi1 phi2 -> holds true phi1 phi2.
+
+Theorem soundness (A : system cfg) env (phi1 phi2 : formula cfg env) :
+  IS cfg S None A env phi1 phi2 ->
+  system_holds A ->
+  holds false phi1 phi2.
+Proof.
+intros pf HA.
+apply approx_holds.
+intro i.
+apply (ExPathSoundness.soundness pf);trivial.
+clear -HA i.
+pose proof holds_approx.
+unfold ExPathSoundness.system_holds;intros.
+eauto.
+Qed.
