coq/mixed_shallow/generic_soundness.v
@@ -1,0 +1,210 @@
+Add LoadPath "../ml_proof".
+
+Require Import Wellfounded.
+Require Import reduction.
+
+Require Import proofsystem.
+Set Implicit Arguments.
+
+Lemma clos_true_step : forall {A: Set} (R : A -> A -> Prop) x z, clos R true x z ->
+                                   exists y, R x y /\ clos R false y z.
+intros.
+rewrite clos_iff_left in H;inversion H;subst;rewrite <- ?clos_iff_left in * |-;
+eauto using clos_refl, clos_unstrict.
+Qed.
+
+Module Type ReachabilitySemantics.
+  Parameter cfg : Set.
+  Parameter S : cfg -> cfg -> Prop.
+
+  Parameter index : Set.
+  (* This is one step of soundness relation *)
+  Parameter ix_rel : index -> index -> Prop.
+
+  Parameter holds : bool -> forall env, 
+                      formula cfg env -> formula cfg env->
+                      index -> Prop.
+
+  (*
+  Parameter ix_wf : well_founded (fun x y => ix_rel y x).
+   *)
+
+  (* Will this lemma be any harder to supply than one that
+     distinguishes a one-step and all-step version of ix_rel,
+     and only promises immediate successors in the
+     argument of the hypothesis? *)
+  Parameter ix_rel_ind : forall env (phi phi' : formula cfg env),
+      forall i0,
+      (forall i, clos ix_rel false i0 i ->
+                   (forall i', ix_rel i i' -> holds true phi phi' i') ->
+                   holds true phi phi' i)
+       -> holds true phi phi' i0.
+
+  Parameter holds_strict_later : forall env phi1 phi2 i,
+                                   @holds true env phi1 phi2 i ->
+                                   forall i', ix_rel i i' ->
+                                   holds true phi1 phi2 i'.
+
+  Parameter holds_unstrict : forall env phi1 phi2 i,
+                           @holds true env phi1 phi2 i -> holds false phi1 phi2 i.
+
+
+  Parameter holds_step : forall env (phi phi' : formula cfg env),
+    (forall (e : env) (c : cfg),
+      phi e c ->
+      (exists c2 : cfg, S c c2) /\ (forall c2 : cfg, S c c2 -> phi' e c2)) ->
+    forall i, holds true phi phi' i.
+  Parameter holds_refl : forall env phi i, @holds false env phi phi i.
+
+  Parameter holds_trans_strict : forall env phi phi' phi'' i,
+    @holds true env phi phi' i ->
+    (forall i' : index, ix_rel i i' -> holds false phi' phi'' i') ->
+   holds true phi phi'' i.
+  Parameter holds_trans : forall env phi phi' phi'' i,
+    @holds false env phi phi' i ->
+    holds false phi' phi'' i ->
+    holds false phi phi'' i.
+
+  Parameter holds_case :
+    forall strict env (phi phi1 phi' : formula cfg env) i,
+      holds strict phi phi' i -> holds strict phi1 phi' i ->
+      holds strict (fun (e : env) (g : cfg) => phi e g \/ phi1 e g) phi' i.
+
+  Parameter holds_mut_conseq :
+    forall strict env1 (phi1 phi2 : formula cfg env1)
+                  env2 (phi1' phi2' : formula cfg env2),
+     (forall gamma rho,
+        phi1 rho gamma ->
+        exists rho', phi1' rho' gamma /\
+                     forall gamma', phi2' rho' gamma' -> phi2 rho gamma') ->
+    forall i, holds strict phi1' phi2' i ->
+              holds strict phi1 phi2 i.
+
+End ReachabilitySemantics.
+
+Module Soundness(Sem : ReachabilitySemantics).  
+  Import Sem.
+
+  Definition system_holds (S : system cfg) (i : index) : Prop :=
+    forall env phi1 phi2, S env phi1 phi2 -> holds true phi1 phi2 i.
+
+  Lemma system_next (S : system cfg) (i : index) :
+    system_holds S i -> forall i', ix_rel i i' -> system_holds S i'.
+  Proof. unfold system_holds; eauto using holds_strict_later. Qed.
+
+  Lemma system_later (S : system cfg) (i : index) :
+    system_holds S i -> forall i', clos ix_rel false i i' -> system_holds S i'.
+  Proof. intros Hsys i' Hpath; revert Hsys; induction Hpath; eauto using system_next. Qed.
+ 
+  Lemma holds_weak : forall (C : option (system cfg)) env phi1 phi2 i,
+                       @holds true env phi1 phi2 i ->
+                       holds
+                       (match C with
+                         | None => false
+                         | Some _ => true
+                       end) phi1 phi2 i.
+  Proof.
+    destruct C;auto using holds_unstrict.
+  Qed.
+
+  Lemma holds_conseq : forall strict env (phi1 phi2 phi1' phi2' : formula cfg env),
+    forall env (phi1 phi2 phi1' phi2' : formula cfg env),
+    (forall rho gamma, phi1 rho gamma -> phi1' rho gamma) ->
+    (forall rho gamma, phi2' rho gamma -> phi2 rho gamma) ->
+    forall i, holds strict phi1' phi2' i ->
+              holds strict phi1 phi2 i.
+    intros.
+    revert H1.
+    apply holds_mut_conseq.
+    firstorder.
+  Qed.
+
+    Ltac spec_ih :=
+    let HA := fresh "HA" in
+    let HC := fresh "HC" in
+    intros ? HA HC;
+    match goal with
+      | [IHcirc : appcontext C [cons_opt_system] |-_] => idtac
+      | _ => repeat match goal with
+                        [IH : forall i, system_holds _ i -> _ |- _] =>
+                        specialize (IH _ HA HC)
+                    end
+    end.
+
+  Lemma soundness : forall C A env phi1 phi2,
+                      IS cfg S C A env phi1 phi2 ->
+                      forall (i : index),
+                        system_holds A i ->
+                        match C with
+                          | None => True
+                          | Some S' => forall i', ix_rel i i' -> system_holds S' i'
+                        end ->
+                        holds (
+                        match C with
+                          | None => false
+                          | Some _ => true
+                        end) phi1 phi2 i.
+  Proof.
+  induction 1;spec_ih.
+  + (* step *)
+    auto using holds_weak, holds_step.
+  + (* axiom *)
+    auto using holds_weak.
+  + (* refl *)
+    destruct C;[destruct H|]; auto using holds_refl.
+  + (* trans *)
+    destruct C.
+    * assert (forall i', ix_rel i i' -> holds false phi' phi'' i') as IH2.
+        clear -IHIS2 HA HC.
+        intros. apply IHIS2;[clear IHIS2|exact I].
+        assert (system_holds A i') by (eauto using system_next).
+        firstorder.
+      clear -IHIS1 IH2.
+      eauto using holds_trans_strict.
+    * assert (holds false phi' phi'' i) as IH2 by (clear -IHIS2 HA HC; auto).
+      clear -IHIS1 IH2.
+      eauto using holds_trans.
+  + (* consequence *)
+    eauto using holds_conseq.
+  + (* case *)
+    auto using holds_case.
+  + (* abstr *)
+    revert IHIS;clear;apply holds_mut_conseq;firstorder.
+  + (* circularity *)
+    apply holds_weak.
+    apply ix_rel_ind.
+    intros i0 Hii0 IHlater.
+    apply IHIS; clear H IHIS.
+    eauto using system_later.
+    simpl.
+    intros i' Hi'.
+    unfold system_holds.
+    intros rho phi1 phi2 H.
+    destruct H.
+    * (* rules from C *)
+      destruct C;[|solve[destruct H]].
+      simpl in H.
+      assert (forall i', clos ix_rel true i i' -> system_holds s i').
+        clear -HC. intros.
+        apply clos_true_step in H.
+        destruct H as [i1 [Hstep Hrest]].
+        eauto using system_later.
+      clear HC; rename H0 into HC.
+      assert (clos ix_rel true i i').
+        clear -Hi' Hii0.
+        eauto using clos, clos_cons_rt.
+      specialize (HC _ H0).
+      auto.
+    * (* The added rule *)
+      destruct H as [-> [-> ->]].
+      unfold eq_rect_r in * |- *; simpl eq_rect in * |- *.
+      auto.
+  + (* subst *)
+    eauto using holds_mut_conseq.
+  + (* Logical framing *)
+    revert IHIS;
+    eapply holds_mut_conseq;
+    intuition;
+    eauto.
+  Qed.
+End Soundness.
